src/specs/effects.fst
@@ -3,49 +3,47 @@
 --*)
 
 // $legal:614:
-// 
+//
 // Copyright 2015 Michael Lowell Roberts
-// 
+//
 // Licensed under the Apache License, Version 2.0 (the "License");
 // you may not use this file except in compliance with the License.
 // You may obtain a copy of the License at
-// 
+//
 //     http://www.apache.org/licenses/LICENSE-2.0
-// 
+//
 // Unless required by applicable law or agreed to in writing, software
 // distributed under the License is distributed on an "AS IS" BASIS,
 // WITHOUT WARRANTIES OR CONDITIONS OF ANY KIND, either express or implied.
 // See the License for the specific language governing permissions and
 // limitations under the License.
-// 
+//
 // ,$
-
-//@requires "seq.fst"
 
 module Tesseract.Specs.Effects
 
    type region_id_t = nat
 
    type step_g (state_t: Type) (step_kind_t: Type)
-      = region_id_t 
+      = region_id_t
          -> state_t
-         -> step_kind_t 
+         -> step_kind_t
          -> Tot (state_t * (Seq.State (region_id_t * step_kind_t)))
 
-   type effect_g (state_t: Type) (step_kind_t: Type) 
+   type effect_g (state_t: Type) (step_kind_t: Type)
       =
-      | Spawn: 
+      | Spawn:
           state0: state_t
          -> step: step_g state_t step_kind_t
          -> effect_g state_t step_kind_t
-      | Step: 
+      | Step:
          region_id: region_id_t
-         -> step_kind: step_kind_t 
+         -> step_kind: step_kind_t
          -> effect_g state_t step_kind_t
 
-   type _log_g 
-      (state_t: Type) 
-      (step_kind_t: Type) 
+   type _log_g
+      (state_t: Type)
+      (step_kind_t: Type)
       = Seq.State (effect_g state_t step_kind_t)
 
 // $vim-fst:32: vim:set sts=3 sw=3 et ft=fstar:,$
