src/specs/set.fst
@@ -1,41 +1,41 @@
 // $legal:614:
-// 
+//
 // Copyright 2015 Michael Lowell Roberts
-// 
+//
 // Licensed under the Apache License, Version 2.0 (the "License");
 // you may not use this file except in compliance with the License.
 // You may obtain a copy of the License at
-// 
+//
 //     http://www.apache.org/licenses/LICENSE-2.0
-// 
+//
 // Unless required by applicable law or agreed to in writing, software
 // distributed under the License is distributed on an "AS IS" BASIS,
 // WITHOUT WARRANTIES OR CONDITIONS OF ANY KIND, either express or implied.
 // See the License for the specific language governing permissions and
 // limitations under the License.
-// 
+//
 // ,$
 
 module Tesseract.Specs.Set
 
-   type set_g (item_t: Type) 
+   type set_g (item_t: Type)
       = item_t -> Tot bool
 
    val empty: #item_t: Type -> Tot (set_g item_t)
-   let empty (item_t: Type) 
+   let empty (item_t: Type)
       = fun _ -> false
 
-   val is_mem: 
-      #item_t: Type 
-      -> set_g item_t 
-      -> item_t 
+   val is_mem:
+      #item_t: Type
+      -> set_g item_t
+      -> item_t
       -> Tot bool
    let is_mem set = set
 
-   val add: 
-      #item_t: Type 
-      -> set: set_g item_t 
-      -> item: item_t{not (is_mem set item)} 
+   val add:
+      #item_t: Type
+      -> set: set_g item_t
+      -> item: item_t{not (is_mem set item)}
       -> Tot (set_g item_t)
    let add (item_t: Type) set item
       = fun i ->
@@ -43,6 +43,5 @@ module Tesseract.Specs.Set
                true
             else
                set i
-             
 
 // $vim-fst:32: vim:set sts=3 sw=3 et ft=fstar:,$
